finished conversion to Utf8

theories/semantics.v
@@ -16,29 +16,29 @@ Set Implicit Arguments.
 
 Section semantics.
 
-  Implicit Types (P Q : term -> Prop).
+  Implicit Types (P Q : term → Prop).
 
-  Definition sem_arrow P Q t := forall u, P u -> Q (t @ u). 
+  Definition sem_arrow P Q t := ∀u, P u → Q (t @ u). 
 
   Notation " P ~> Q " := (@sem_arrow P Q) (at level 68).
 
-  Fact sem_arrow_mono P P' Q Q' : P' ⊆₁ P -> Q ⊆₁ Q' -> P~>Q ⊆₁ P'~>Q'.
+  Fact sem_arrow_mono P P' Q Q' : P' ⊆₁ P → Q ⊆₁ Q' → P~>Q ⊆₁ P'~>Q'.
   Proof. intros HP HQ ? Hu ? Ht; apply HQ, Hu, HP, Ht. Qed.
 
-  Notation "P ≡ Q" := (forall u, P u <-> Q u) (at level 70).
+  Notation "P ≡ Q" := (∀u, P u ↔ Q u) (at level 70).
 
-  Fact sem_arrow_congr P P' Q Q' : P ≡ P' -> Q ≡ Q' -> P~>Q ≡ P'~>Q'.
+  Fact sem_arrow_congr P P' Q Q' : P ≡ P' → Q ≡ Q' → P~>Q ≡ P'~>Q'.
   Proof. intros H1 H2 u; split; apply sem_arrow_mono; apply H1 || apply H2. Qed.
 
   Local Definition N := term_beta_sn.
   
   (* Saturation look like an inductive rule under which pre-models must be closed*) 
-  Local Definition Nsaturated P := forall u a l, N a -> P (u⌈a⌉@*l) -> P ((Ⲗ u)@*(a::l)).
+  Local Definition Nsaturated P := ∀ u a l, N a → P (u⌈a⌉@*l) → P ((Ⲗ u@a)@*l).
 
   Local Fact Nsaturated_N : Nsaturated N.
   Proof. intros ? ? ?; apply term_beta_sn_app. Qed.
 
-  Local Fact Nsaturated_right P Q : Nsaturated Q -> Nsaturated (P~>Q).
+  Local Fact Nsaturated_right P Q : Nsaturated Q → Nsaturated (P~>Q).
   Proof.
     intros HQ u a l Ha H q Hq.
     change (Q ((Ⲗ u)@*(a::l)@*(q::nil))).
@@ -50,14 +50,14 @@ Section semantics.
   Qed.
 
   (* Nsaturated is stable under intersections *)
-  Local Fact Nsaturated_cap X (Q : X -> Prop) (f : X -> term -> Prop) :
-         (forall x, Q x -> Nsaturated (f x))
-      -> Nsaturated (fun u => forall x, Q x -> f x u).
+  Local Fact Nsaturated_cap X (Q : X → Prop) (f : X → term → Prop) :
+         (∀x, Q x → Nsaturated (f x))
+       → Nsaturated (λ u, ∀x, Q x → f x u).
   Proof. intros H u a l H1 H2 ? ?; apply H; eauto. Qed. 
 
-  Local Definition N0 u := exists x l, u = £x @* l /\ Forall N l.
+  Local Definition N0 u := ∃ x l, u = £x @* l ∧ Forall N l.
 
-  Local Fact N0_N_app u v : N0 u -> N v -> N0 (u@v).
+  Local Fact N0_N_app u v : N0 u → N v → N0 (u@v).
   Proof.
     intros (x & l & -> & H1) H2.
     exists x, (l++[v]); rewrite term_app_snoc; split; eauto.
@@ -78,9 +78,9 @@ Section semantics.
 
   Local Definition Nadapted P :=
             Nsaturated N
-         /\ P ⊆₁ N~>P /\ N~>P ⊆₁ P~>N /\ P~>N ⊆₁ N.
+          ∧ P ⊆₁ N~>P ∧ N~>P ⊆₁ P~>N ∧ P~>N ⊆₁ N.
 
-  Local Fact Nsaturated_N0 : ~ Nsaturated N0.
+  Local Fact Nsaturated_N0 : ¬ Nsaturated N0.
   Proof.
     intros C.
     destruct (C (£0) (£0) []) as (x & l & H1 & _); simpl.
@@ -107,25 +107,23 @@ Section semantics.
       now intros []%term_beta_sn_inv.
   Qed.
 
-  Local Definition Nmodel P := Nsaturated P /\ N0 ⊆₁ P /\ P ⊆₁ N.
+  Local Definition Nmodel P := Nsaturated P ∧ N0 ⊆₁ P ∧ P ⊆₁ N.
 
   Local Fact Nmodel_N : Nmodel N.
   Proof. split; [ | split ]; auto. Qed.
 
   Hint Resolve Nmodel_N : core.
 
-  Fixpoint type_sem (A : type) (I : nat -> term -> Prop) : term -> Prop :=
+  Fixpoint type_sem (A : type) (I : nat → term → Prop) : term → Prop :=
     match A with
     | £ x => I x
     | A⇨B => type_sem A I ~> type_sem B I
-    | ∇ A => fun u => forall P, Nmodel P -> type_sem A (P∷I) u
+    | ∇ A => λ u, ∀P, Nmodel P → type_sem A (P∷I) u
     end.
 
   Hint Resolve in_or_app : core.
 
-  Fact type_sem_ext A I J : 
-           (forall x, x ∈ syn_vars A -> I x ≡ J x) 
-        -> type_sem A I ≡ type_sem A J. 
+  Fact type_sem_ext A I J : (∀x, x ∈ 𝓥 A → I x ≡ J x) → type_sem A I ≡ type_sem A J. 
   Proof.
     induction A as [ x | A IHA B IHB | A IHA ] in I, J |- *; simpl; intros H u.
     + apply H; simpl; eauto.
@@ -140,7 +138,7 @@ Section semantics.
   Qed.
 
   Fact type_sem_Nmodel A I : 
-         (forall x, x ∈ syn_vars A -> Nmodel (I x)) -> Nmodel (type_sem A I).
+         (∀x, x ∈ 𝓥 A → Nmodel (I x)) → Nmodel (type_sem A I).
   Proof.
     induction A as [ x | A IHA B IHB | A IHA ] in I |- *; simpl; intros H; eauto.
     + split; [ | split ].
@@ -166,8 +164,7 @@ Section semantics.
         intros [] ?; simpl; auto; now apply H, In_list_pred.
   Qed.
 
-  Fact type_sem_ren A I f : 
-         type_sem (syn_ren A f) I ≡ type_sem A (fun x => I (f x)).
+  Fact type_sem_ren A I f : type_sem A⟬f⟭ I ≡ type_sem A (I⋄f).
   Proof.
     induction A as [ x | A IHA B IHB | A IHA ] in I, f |- *; simpl; intros u; try easy.
     + apply sem_arrow_congr; auto.
@@ -182,8 +179,7 @@ Section semantics.
         revert H; apply type_sem_ext; now intros [].
   Qed.
 
-  Fact type_sem_subst A I f : 
-         type_sem (syn_subst A f) I ≡ type_sem A (fun x => type_sem (f x) I).
+  Fact type_sem_subst A I f : type_sem A⟪f⟫ I ≡ type_sem A (λ x, type_sem (f x) I).
   Proof.
     induction A as [ x | A IHA B IHB | A IHA ] in I, f |- *; simpl; intros u; try easy.
     + apply sem_arrow_congr; auto.
@@ -213,10 +209,10 @@ Section semantics.
  
   Theorem FTJ_adequacy Γ u A :
         Γ ⊢ u ∶ A
-     -> forall I f,
-            (forall x, (* x ∈ syn_vars A \/ x ∈ syn_vars (Γ n) -> *) Nmodel (I x))
-         -> (forall n, n ∈ syn_vars u -> type_sem (Γ n) I (f n))
-         -> type_sem A I (syn_subst u f).
+      → ∀ I f,
+            (∀x, (* x ∈ syn_vars A \/ x ∈ syn_vars (Γ n) → *) Nmodel (I x))
+          → (∀n, n ∈ 𝓥 u → type_sem (Γ n) I (f n))
+          → type_sem A I u⟪f⟫.
   Proof.
     induction 1 as [ G x | G u A B H1 IH1 | G u v A B H1 IH1 H2 IH2 | G u A H1 IH1 | G u A B H1 IH1 ];
       simpl; intros I f HI Hf; eauto.
@@ -247,9 +243,9 @@ Section semantics.
      then u belongs to the model of type A *)
 
   Theorem FTJ_adequacy' Γ u A I :
-           (forall x, Nmodel (I x))
-        -> (forall n, n ∈ syn_vars u -> type_sem (Γ n) I (£ n))
-        -> Γ ⊢ u ∶ A -> type_sem A I u.
+           (∀x, Nmodel (I x))
+         → (∀n, n ∈ 𝓥 u → type_sem (Γ n) I (£ n))
+         → Γ ⊢ u ∶ A → type_sem A I u.
   Proof.
     intros H1 H2 H.
     rewrite <- syn_subst_id.
@@ -257,7 +253,7 @@ Section semantics.
   Qed.
 
   (* Strong Normalization for Curry-style system F *)
-  Theorem FTJ_beta_sn Γ u A : Γ ⊢ u ∶ A -> term_beta_sn u.
+  Theorem FTJ_beta_sn Γ u A : Γ ⊢ u ∶ A → term_beta_sn u.
   Proof.
     intros H.
     apply FTJ_adequacy' with (I := fun _ => N) in H; auto.
@@ -268,7 +264,7 @@ Section semantics.
       * now exists x, [].
   Qed.
 
-  Definition N1 u := N u /\ syn_vars u <> [].
+  Definition N1 u := N u ∧ 𝓥 u ≠ [].
 
   Fact Nmodel_N1 : Nmodel N1.
   Proof.
@@ -277,7 +273,7 @@ Section semantics.
       contradict H3.
       rewrite term_app_vars in H3 |- *; simpl in H3 |- *.
       generalize (syn_replace_vars u a).
-      apply app_eq_nil in H3 as (-> & (-> & ->)%app_eq_nil).
+      apply app_eq_nil in H3 as ((-> & ->)%app_eq_nil & ->).
       rewrite <- !app_nil_end.
       destruct (syn_vars (u⌈a⌉)) as [ | n ]; auto.
       intros C; destruct (C n); simpl; auto.
@@ -298,7 +294,7 @@ Section semantics.
   Qed.
 
   (* A term of type ∀£0 (bottom) cannot be closed *)
-  Theorem FTJ_bot Γ u : Γ ⊢ u ∶ ∇£0 -> 𝓥 u <> [].
+  Theorem FTJ_bot Γ u : Γ ⊢ u ∶ ∇£0 → 𝓥 u ≠ [].
   Proof.
     intros H.
     apply (@type_sem_bot (fun _ => N)), FTJ_adequacy' with (3 := H); auto.
