theories/utils.v
@@ -7,23 +7,23 @@
 (*        Mozilla Public License Version 2.0, MPL-2.0         *)
 (**************************************************************)
 
-From Coq Require Import List Relations Wellfounded.
+From Coq Require Import List Relations Wellfounded Utf8.
 Import ListNotations.
 
 Set Implicit Arguments.
 
 #[global] Infix "∈" := In (at level 70, no associativity).
 
-#[global] Notation rinv R := (fun x y => R y x).
-#[global] Notation "P '⊆₁' Q" := (forall x, P x -> Q x) (at level 70).
+#[global] Notation rinv R := (λ x y, R y x).
+#[global] Notation "P '⊆₁' Q" := (∀x, P x → Q x) (at level 70, format "P  ⊆₁  Q").
 
 Arguments clos_trans {_}.
 Arguments clos_refl_trans {_}.
 
-Theorem list_snoc_rect X (P : list X -> Type) :
+Theorem list_snoc_rect X (P : list X → Type) :
           P []
-       -> (forall l x, P l -> P (l++[x]))
-       -> forall l, P l.
+       → (∀ l x, P l → P (l++[x]))
+       → ∀l, P l.
 Proof.
   intros H1 H2 l; revert P H1 H2.
   induction l as [ | x l IHl ]; eauto.
@@ -37,46 +37,48 @@ Section closure_t_rt.
 
   Variables (X : Type).
 
-  Implicit Type (R : X -> X -> Prop).
+  Implicit Type (R : X → X → Prop).
 
   Hint Constructors clos_trans clos_refl_trans : core.
 
-  Local Fact clos_trans_rev' R x y : clos_trans R x y -> clos_trans (rinv R) y x.
+  Local Fact clos_trans_rev' R x y : clos_trans R x y → clos_trans (rinv R) y x.
   Proof. induction 1; eauto. Qed.
 
-  Fact clos_trans_rinv R x y : clos_trans R x y <-> clos_trans (rinv R) y x.
+  Fact clos_trans_rinv R x y : clos_trans R x y ↔ clos_trans (rinv R) y x.
   Proof. split; now intros ?%clos_trans_rev'. Qed.
 
-  Local Fact clos_refl_trans_rev' R x y : clos_refl_trans R x y -> clos_refl_trans (rinv R) y x.
+  Local Fact clos_refl_trans_rev' R x y : clos_refl_trans R x y → clos_refl_trans (rinv R) y x.
   Proof. induction 1; eauto. Qed.
 
-  Fact clos_refl_trans_rinv R x y : clos_refl_trans R x y <-> clos_refl_trans (rinv R) y x.
+  Fact clos_refl_trans_rinv R x y : clos_refl_trans R x y ↔ clos_refl_trans (rinv R) y x.
   Proof. split; now intros ?%clos_refl_trans_rev'. Qed.
 
+(*
   Fact clos_refl_trans_clos_trans R x y :
-      clos_refl_trans R x y -> x = y \/ clos_trans R x y.
+      clos_refl_trans R x y → x = y ∨ clos_trans R x y.
   Proof. induction 1 as [ | | x y z _ [] _ [] ]; subst; eauto. Qed.
+*)
 
   Fact clos_trans_fun R f :
-         (forall x y, R x y -> R (f x) (f y))
-      -> (forall x y, clos_trans R x y -> clos_trans R (f x) (f y)).
+         (∀ x y, R x y → R (f x) (f y))
+       → (∀ x y, clos_trans R x y → clos_trans R (f x) (f y)).
   Proof. induction 2; eauto. Qed.
 
   Fact clos_refl_trans_fun R f :
-         (forall x y, R x y -> R (f x) (f y))
-      -> (forall x y, clos_refl_trans R x y -> clos_refl_trans R (f x) (f y)).
+         (∀ x y, R x y → R (f x) (f y))
+       → (∀ x y, clos_refl_trans R x y → clos_refl_trans R (f x) (f y)).
   Proof. induction 2; eauto. Qed.
 
 End closure_t_rt.
 
 #[local] Hint Resolve Acc_intro Acc_inv : core.
 
-Fact Acc_inv_clos_refl_trans X (R : X -> X -> Prop) x y :
-     clos_refl_trans R y x -> Acc R x -> Acc R y.
+Fact Acc_inv_clos_refl_trans X (R : X → X → Prop) x y :
+     clos_refl_trans R y x → Acc R x → Acc R y.
 Proof. induction 1; eauto. Qed.
 
-Fact Acc_inv_clos_refl_trans_rinv X (R : X -> X -> Prop) x y :
-       clos_refl_trans R x y -> Acc (rinv R) x -> Acc (rinv R) y.
+Fact Acc_inv_clos_refl_trans_rinv X (R : X → X → Prop) x y :
+       clos_refl_trans R x y → Acc (rinv R) x → Acc (rinv R) y.
 Proof.
   intros H1%clos_refl_trans_rinv.
   now apply Acc_inv_clos_refl_trans.
@@ -85,36 +87,36 @@ Qed.
 Section Acc_lex_product_rect.
 
   Variables (X Y : Type) 
-            (R : X -> X -> Prop) 
-            (T : Y -> Y -> Prop)
-            (P : X -> Y -> Type).
+            (R : X → X → Prop) 
+            (T : Y → Y → Prop)
+            (P : X → Y → Type).
 
   Hint Resolve Acc_inv Acc_intro : core.
 
   Section Acc_lex_rect.
 
-    Hypothesis (HP : forall x y, 
-                      Acc R x 
-                   -> Acc T y 
-                   -> (forall x' y', R x' x -> Acc T y' -> P x' y')
-                   -> (forall y', T y' y -> P x y')
-                   -> P x y).
+    Hypothesis (HP : ∀ x y, 
+                     Acc R x 
+                   → Acc T y 
+                   → (∀ x' y', R x' x → Acc T y' → P x' y')
+                   → (∀ y', T y' y → P x y')
+                   → P x y).
 
-    Theorem Acc_lex_rect x y : Acc R x -> Acc T y -> P x y.
+    Theorem Acc_lex_rect x y : Acc R x → Acc T y → P x y.
     Proof. induction 1 in y |- *; induction 1; eauto. Qed.
 
   End Acc_lex_rect.
 
   Section Acc_product_rect.
 
-    Hypothesis (HP : forall x y, 
-                      Acc R x 
-                   -> Acc T y 
-                   -> (forall x', R x' x -> P x' y)
-                   -> (forall y', T y' y -> P x y')
-                   -> P x y).
+    Hypothesis (HP : ∀ x y, 
+                     Acc R x 
+                   → Acc T y 
+                   → (∀x', R x' x → P x' y)
+                   → (∀y', T y' y → P x y')
+                   → P x y).
 
-    Theorem Acc_product_rect x y : Acc R x -> Acc T y -> P x y.
+    Theorem Acc_product_rect x y : Acc R x → Acc T y → P x y.
     Proof. intros Hx; revert Hx y; do 2 induction 1; apply HP; eauto. Qed.
 
   End Acc_product_rect.
@@ -123,16 +125,16 @@ End Acc_lex_product_rect.
 
 Section Acc_rinv_fun_rect.
 
-  Variables (X Y : Type) (R : Y -> Y -> Prop) (f g : X -> Y)
-            (P : Y -> Type)
-            (HP : forall x, Acc (rinv R) (f x)
-                         -> (forall x', R (f x) (f x') -> P (g x'))
-                         -> P (g x)).
+  Variables (X Y : Type) (R : Y → Y → Prop) (f g : X → Y)
+            (P : Y → Type)
+            (HP : ∀x, Acc (rinv R) (f x)
+                    → (∀x', R (f x) (f x') → P (g x'))
+                    → P (g x)).
 
-  Local Lemma Acc_rinv_fun_rect_eq y : Acc (rinv R) y -> forall x, y = f x -> P (g x).
+  Local Lemma Acc_rinv_fun_rect_eq y : Acc (rinv R) y → ∀x, y = f x → P (g x).
   Proof. induction 1; intros ? ->; eauto. Qed.
 
-  Theorem Acc_rinv_fun_rect x : Acc (rinv R) (f x) -> P (g x).
+  Theorem Acc_rinv_fun_rect x : Acc (rinv R) (f x) → P (g x).
   Proof. intros; eapply Acc_rinv_fun_rect_eq; eauto. Qed.
 
 End Acc_rinv_fun_rect.
@@ -143,31 +145,31 @@ Section Acc_rinv_lex_fun_rect.
       designed to establish the following result called
       term_beta_sn_app in beta.v:
 
-           SN a -> SN (u⌈a⌉ @ *m) -> SN (λ u @* a::m)
+           SN a → SN (u⌈a⌉ @ *m) → SN (λ u @* a::m)
 
       where f and g are instantiated as 
             f a u m := u⌈a⌉ @ *m 
         and g a u m := λ u @* a::m
       and P is just SN := Acc (rinv term_beta) *)
 
-  Variables (X Y Z K : Type) (R : X -> X -> Prop) (T : K -> K -> Prop)
-            (f g : X -> Y -> Z -> K)
-            (P : K -> Type)
-            (HP : forall x y z,
-                     Acc (rinv R) x
-                  -> Acc (rinv T) (f x y z)
-                  -> (forall x' y' z', R x x' -> Acc (rinv T) (f x' y' z') -> P (g x' y' z'))
-                  -> (forall y' z', T (f x y z) (f x y' z') -> P (g x y' z'))
-                  -> P (g x y z)).
+  Variables (X Y Z K : Type) (R : X → X → Prop) (T : K → K → Prop)
+            (f g : X → Y → Z → K)
+            (P : K → Type)
+            (HP : ∀ x y z,
+                    Acc (rinv R) x
+                  → Acc (rinv T) (f x y z)
+                  → (∀ x' y' z', R x x' → Acc (rinv T) (f x' y' z') → P (g x' y' z'))
+                  → (∀ y' z', T (f x y z) (f x y' z') → P (g x y' z'))
+                  → P (g x y z)).
 
   Local Lemma Acc_lex_fun_rect_eq x k :
-      Acc (rinv R) x -> Acc (rinv T) k -> forall y z, k = f x y z -> P (g x y z).
+      Acc (rinv R) x → Acc (rinv T) k → ∀ y z, k = f x y z → P (g x y z).
   Proof.
     intros H1 H2; pattern x, k; revert x k H1 H2; apply Acc_lex_rect.
     intros; subst; eauto.
   Qed.
 
-  Theorem Acc_rinv_lex_fun_rect x y z : Acc (rinv R) x -> Acc (rinv T) (f x y z) -> P (g x y z).
+  Theorem Acc_rinv_lex_fun_rect x y z : Acc (rinv R) x → Acc (rinv T) (f x y z) → P (g x y z).
   Proof. intros; eapply Acc_lex_fun_rect_eq; eauto. Qed.
 
 End Acc_rinv_lex_fun_rect.
@@ -180,33 +182,31 @@ Section prod_list.
 
   Variables (X : Type).
 
-  Implicit Type (R : X -> X -> Prop).
+  Implicit Type (R : X → X → Prop).
 
-  Inductive prod_list R : list X -> list X -> Prop :=
-    | in_prod_list l x y r : R x y -> prod_list R (l++x::r) (l++y::r).
-
-  Notation Π := prod_list.
+  Inductive prod_list R : list X → list X → Prop :=
+    | in_prod_list l x y r : R x y → prod_list R (l++x::r) (l++y::r).
 
   Hint Constructors prod_list : core.
 
   (* We implement a right inversion lemma for prod_list
      using a custom inversion predicate (called telescope ?) *)
 
-  Inductive prod_list_cons_right R y m : list X -> Prop :=
-    | in_prod_list_cons_right_0 x : R x y -> prod_list_cons_right R y m (x::m)
-    | in_prod_list_cons_right_1 l : Π R l m -> prod_list_cons_right R y m (y::l).
+  Inductive prod_list_cons_right R y m : list X → Prop :=
+    | in_prod_list_cons_right_0 x : R x y → prod_list_cons_right R y m (x::m)
+    | in_prod_list_cons_right_1 l : prod_list R l m → prod_list_cons_right R y m (y::l).
 
   Hint Constructors prod_list_cons_right : core.
 
   Local Fact prod_list_right_inv R l m :
-          Π R l m 
-       -> match m with
+          prod_list R l m 
+        → match m with
           | []   => False
           | y::m => prod_list_cons_right R y m l
           end.
   Proof. intros [[]]; simpl; eauto. Qed. 
 
-  Lemma prod_list_Acc R l : Forall (Acc R) l -> Acc (Π R) l.
+  Lemma prod_list_Acc R l : Forall (Acc R) l → Acc (prod_list R) l.
   Proof. 
     induction 1 as [ | y m Hy _ IHm ].
     + constructor; now intros ? ?%prod_list_right_inv.
