theories/typing.v
@@ -33,7 +33,7 @@ where "Γ ⊢ u ∶ A" := (F_Typing_Judgement Γ u A).
 
 #[global] Hint Constructors F_Typing_Judgement : core.
 
-Fact FTJ_var Γ n A : Γ n = A -> Γ ⊢ £n ∶ A.
+Fact FTJ_var Γ n A : Γ n = A → Γ ⊢ £n ∶ A.
 Proof. intros <-; constructor. Qed.
 
 #[global] Hint Resolve FTJ_var : core.
@@ -46,10 +46,7 @@ Proof. do 2 constructor; eauto. Qed.
 
 #[local] Hint Resolve in_or_app in_eq in_cons : core.
 
-Fact FTJ_ext Γ Δ u A :
-       (forall x, x ∈ syn_vars u -> Γ x = Δ x)
-     -> Γ ⊢ u ∶ A
-     -> Δ ⊢ u ∶ A.
+Fact FTJ_ext Γ Δ u A : (∀x, x ∈ 𝓥 u → Γ x = Δ x) → Γ ⊢ u ∶ A → Δ ⊢ u ∶ A.
 Proof.
   intros H.
   induction 1 as [ G x | G u A B H1 IH1 | G u v A B H1 IH1 H2 IH2 | G u A H1 IH1 | G u A B H1 IH1 ]
@@ -66,9 +63,7 @@ Proof.
 Qed.
 
 (* F typing judgements are closed under substituion of types *)
-Fact FTJ_type_subst Γ u A f :
-          Γ ⊢ u ∶ A
-       -> (fun x => syn_subst (Γ x) f) ⊢ u ∶ syn_subst A f.
+Fact FTJ_type_subst Γ u A f : Γ ⊢ u ∶ A → (λ x, (Γ x)⟪f⟫) ⊢ u ∶ A⟪f⟫.
 Proof.
   induction 1 as [ G x | G u A B H1 IH1 | G u v A B H1 IH1 H2 IH2 | G u A H1 IH1 | G u A B H1 IH1 ]
     in f |- *; simpl; eauto.
@@ -87,9 +82,7 @@ Proof.
 Qed.
 
 (* F typing judgements are closed under renaming of types *)
-Fact FTJ_type_ren Γ u A f :
-          Γ ⊢ u ∶ A
-       -> (fun x => syn_ren (Γ x) f) ⊢ u ∶ syn_ren A f.
+Fact FTJ_type_ren Γ u A f : Γ ⊢ u ∶ A → (λ x, (Γ x)⟬f⟭) ⊢ u ∶ A⟬f⟭.
 Proof.
   intros H.
   rewrite syn_ren_eq_subst.
@@ -99,10 +92,7 @@ Proof.
 Qed.
 
 (* F typing judgements are closed under renaming of terms *)
-Fact FTJ_term_ren Γ Δ A u f :
-            Γ ⊢ u ∶ A
-         -> (forall x, x ∈ syn_vars u -> Δ (f x) = Γ x)
-         -> Δ ⊢ syn_ren u f ∶ A.
+Fact FTJ_term_ren Γ Δ A u f : Γ ⊢ u ∶ A → (∀x, x ∈ 𝓥 u → Δ (f x) = Γ x) → Δ ⊢ u⟬f⟭ ∶ A.
 Proof.
   intros H; revert H Δ f.
   induction 1 as [ G x | G u A B H1 IH1 | G u v A B H1 IH1 H2 IH2 | G u A H1 IH1 | G u A B H1 IH1 ];
@@ -116,10 +106,7 @@ Proof.
 Qed.
 
 (* F typing judgements are closed under substitution of terms *)
-Fact FTJ_term_subst Γ Δ C u f :
-            Γ ⊢ u ∶ C
-         -> (forall x, x ∈ syn_vars u -> Δ ⊢ f x ∶ Γ x)
-         -> Δ ⊢ syn_subst u f ∶ C.
+Fact FTJ_term_subst Γ Δ A u f : Γ ⊢ u ∶ A → (∀x, x ∈ 𝓥 u → Δ ⊢ f x ∶ Γ x) → Δ ⊢ u⟪f⟫ ∶ A.
 Proof.
    intros H; revert H Δ f.
    induction 1 as [ G x | G u A B H1 IH1 | G u v A B H1 IH1 H2 IH2 | G u A H1 IH1 | G u A B H1 IH1 ];
@@ -135,8 +122,8 @@ Proof.
 Qed.
 
 (* This one does not hold, see below
-   Fact FTJ_vars_conclusion Γ C u : Γ ⊢ u ∶ C -> forall x, x ∈ syn_vars C -> exists n, n ∈ syn_vars u /\ x ∈ syn_vars (Γ n).
+   Fact FTJ_vars_conclusion Γ C u : Γ ⊢ u ∶ C → ∀x, x ∈ 𝓥 C → exists n, n ∈ 𝓥 u /\ x ∈ 𝓥 (Γ n).
 *)
 
-Fact FTJ_cex_1 : (fun _ => Ⲗ(£0)) ⊢ Ⲗ(£0) ∶ £0⇨£0.
+Fact FTJ_cex_1 : (λ _, Ⲗ(£0)) ⊢ Ⲗ(£0) ∶ £0⇨£0.
 Proof. constructor; constructor 1 with (Γ := £0∷_). Qed.
